adds partially done code for this new proof approach

GenTest-py/Decoding.py
@@ -1,0 +1,78 @@
+import sys
+from typing import Callable, Any, TypeVar, NamedTuple
+from math import floor
+from itertools import count
+
+import module_ as module_
+import _dafny as _dafny
+import System_ as System_
+
+# Module: Decoding
+
+class default__:
+    def  __init__(self):
+        pass
+
+    @staticmethod
+    def ValidLogitsForPrefix(logits, prefix):
+        def lambda0_(forall_var_0_):
+            d_0_t_: _dafny.Seq = forall_var_0_
+            return not ((d_0_t_) in (default__.Parser__AllowedNext(prefix))) or ((d_0_t_) in (logits))
+
+        return _dafny.quantifier((default__.Parser__AllowedNext(prefix)).Elements, True, lambda0_)
+
+
+class ProposalStrategy:
+    @_dafny.classproperty
+    def AllSingletonConstructors(cls):
+        return [ProposalStrategy_ArgMax(), ProposalStrategy_Temperature(), ProposalStrategy_TopK(), ProposalStrategy_Nucleus()]
+    @classmethod
+    def default(cls, ):
+        return lambda: ProposalStrategy_ArgMax()
+    def __ne__(self, __o: object) -> bool:
+        return not self.__eq__(__o)
+    @property
+    def is_ArgMax(self) -> bool:
+        return isinstance(self, ProposalStrategy_ArgMax)
+    @property
+    def is_Temperature(self) -> bool:
+        return isinstance(self, ProposalStrategy_Temperature)
+    @property
+    def is_TopK(self) -> bool:
+        return isinstance(self, ProposalStrategy_TopK)
+    @property
+    def is_Nucleus(self) -> bool:
+        return isinstance(self, ProposalStrategy_Nucleus)
+
+class ProposalStrategy_ArgMax(ProposalStrategy, NamedTuple('ArgMax', [])):
+    def __dafnystr__(self) -> str:
+        return f'Decoding.ProposalStrategy.ArgMax'
+    def __eq__(self, __o: object) -> bool:
+        return isinstance(__o, ProposalStrategy_ArgMax)
+    def __hash__(self) -> int:
+        return super().__hash__()
+
+class ProposalStrategy_Temperature(ProposalStrategy, NamedTuple('Temperature', [])):
+    def __dafnystr__(self) -> str:
+        return f'Decoding.ProposalStrategy.Temperature'
+    def __eq__(self, __o: object) -> bool:
+        return isinstance(__o, ProposalStrategy_Temperature)
+    def __hash__(self) -> int:
+        return super().__hash__()
+
+class ProposalStrategy_TopK(ProposalStrategy, NamedTuple('TopK', [])):
+    def __dafnystr__(self) -> str:
+        return f'Decoding.ProposalStrategy.TopK'
+    def __eq__(self, __o: object) -> bool:
+        return isinstance(__o, ProposalStrategy_TopK)
+    def __hash__(self) -> int:
+        return super().__hash__()
+
+class ProposalStrategy_Nucleus(ProposalStrategy, NamedTuple('Nucleus', [])):
+    def __dafnystr__(self) -> str:
+        return f'Decoding.ProposalStrategy.Nucleus'
+    def __eq__(self, __o: object) -> bool:
+        return isinstance(__o, ProposalStrategy_Nucleus)
+    def __hash__(self) -> int:
+        return super().__hash__()
+
