GenTest-py/GeneratedCSD.py
@@ -1,0 +1,21 @@
+import sys
+from typing import Callable, Any, TypeVar, NamedTuple
+from math import floor
+from itertools import count
+
+import module_ as module_
+import _dafny as _dafny
+import System_ as System_
+import Decoding as Decoding
+import CSD as CSD
+
+# Module: GeneratedCSD
+
+class default__:
+    def  __init__(self):
+        pass
+
+    @staticmethod
+    def GeneratedProgram():
+        return CSD.Program_ReturnParsed(0, CSD.Policy_MaskWithSynCode(CSD.Policy_WithRejection(CSD.Policy_Base(Decoding.ProposalStrategy_Temperature()))))
+
